src/tls/TLSPRF.fst
@@ -1,19 +1,19 @@
 ﻿(* Copyright (C) 2012--2015 Microsoft Research and INRIA *)
 (* STATUS : JK : assumed two arrays because, has to be fixed *)
-
-#light "off"
-
 module TLSPRF
 
 (* Low-level (bytes -> byte) PRF implementations for TLS *)
 
 open Platform.Bytes
+open Hashing.Spec 
 open TLSConstants
 open TLSInfo
-open HashMAC
-open CoreCrypto
+//open HashMAC
+//open CoreCrypto
+
 
 (* SSL3 *)
+(* 17-02-02 deprecated, and not quite typechecking... 
 
 val ssl_prf_int: bytes -> string -> bytes -> Tot bytes
 let ssl_prf_int secret label seed =
@@ -21,6 +21,7 @@ let ssl_prf_int secret label seed =
   let step1 = hash SHA1 allData in
   let allData = secret @| step1 in
   hash MD5 allData
+
 
 val gen_label: int -> Tot string
 let gen_label (i:int) = String.make (i+1) (Char.char_of_int (Char.int_of_char 'A' + i)) 
@@ -36,7 +37,7 @@ let rec apply_prf secret seed nb res n  =
 val ssl_prf: bytes -> bytes -> int -> Tot bytes
 let ssl_prf secret seed nb = apply_prf secret seed nb empty_bytes  0 
 
-// ADL: sring escape probably doesnt work in current F*
+// ADL: string escape probably doesnt work in current F*
 let ssl_sender_client = abytes "\x43\x4C\x4E\x54"
 let ssl_sender_server = abytes "\x53\x52\x56\x52"
 
@@ -64,13 +65,16 @@ let ssl_verifyCertificate hashAlg ms log  =
   let step1 = hash hashAlg forStep1 in
   let forStep2 = ms @| pad2 @| step1 in
   hash hashAlg forStep2
+*)
 
 (* TLS 1.0 and 1.1 *)
 
-val p_hash_int: macAlg -> bytes -> bytes -> int -> int -> bytes -> bytes -> Tot bytes
+val p_hash_int: a:macAlg -> k:lbytes (macKeySize a) -> bytes -> int -> int -> bytes -> bytes -> ST bytes
+  (requires (fun _ -> True))
+  (ensures (fun h0 _ h1 -> FStar.HyperStack.modifies Set.empty h0 h1))
 let rec p_hash_int alg secret seed len it aPrev acc =
-  let aCur = tls_mac alg secret aPrev in
-  let pCur = tls_mac alg secret (aCur @| seed) in
+  let aCur = HashMAC.tls_mac alg secret aPrev in
+  let pCur = HashMAC.tls_mac alg secret (aCur @| seed) in
   if it = 1 then
     let hs = macSize alg in
     let r = len % hs in
@@ -91,8 +95,8 @@ let tls_prf secret label seed len =
   let l_s1 = (l_s+1)/2 in
   let secret1,secret2 = split secret l_s1 in
   let newseed = label @| seed in
-  let hmd5  = p_hash (HMAC(MD5)) secret1 newseed len in
-  let hsha1 = p_hash (HMAC(SHA1)) secret2 newseed len in
+  let hmd5  = p_hash (HMAC MD5) secret1 newseed len in
+  let hsha1 = p_hash (HMAC SHA1) secret2 newseed len in
   xor len hmd5 hsha1 
 
 val tls_finished_label: role -> Tot bytes
@@ -110,7 +114,8 @@ let tls_verifyData ms role data =
   tls_prf ms (tls_finished_label role) (md5hash @| sha1hash) 12
 
 (* TLS 1.2 *)
-val tls12prf: cipherSuite -> bytes -> bytes -> bytes -> int -> Tot bytes
+
+val tls12prf: cipherSuite -> bytes -> bytes -> bytes -> len:nat -> Tot (lbytes len)
 let tls12prf cs ms label data len =
   let prfMacAlg = prfMacAlg_of_ciphersuite cs in
   p_hash prfMacAlg ms (label @| data) len
@@ -118,10 +123,11 @@ let tls12prf cs ms label data len =
 let tls12prf' macAlg ms label data len =
   p_hash macAlg ms (label @| data) len
 
-val tls12VerifyData: cipherSuite -> bytes -> role -> bytes -> Tot bytes
+let verifyDataLen = 12  
+
+val tls12VerifyData: cipherSuite -> bytes -> role -> bytes -> Tot (lbytes verifyDataLen)
 let tls12VerifyData cs ms role data =
   let verifyDataHashAlg = verifyDataHashAlg_of_ciphersuite cs in
-  let verifyDataLen = verifyDataLen_of_ciphersuite cs in
   let hashed = hash verifyDataHashAlg data in
   tls12prf cs ms (tls_finished_label role) hashed verifyDataLen
 
@@ -155,12 +161,11 @@ let prf_hashed (pv, cs) secret label data len =
 let prf' a secret data len =
     match a with
     | PRF_TLS_1p2 label macAlg -> tls12prf' macAlg secret label data len  // typically SHA256 but may depend on CS
-    | PRF_TLS_1p01(label)       -> tls_prf          secret label data len  // MD5 xor SHA1
+    | PRF_TLS_1p01 label         -> tls_prf          secret label data len  // MD5 xor SHA1
     | PRF_SSL3_nested           -> ssl_prf          secret       data len  // MD5(SHA1(...)) for extraction and keygen
     | _ -> Platform.Error.unexpected "[prf'] unreachable pattern match"
 
 //let extract a secret data len = prf a secret extract_label data len
 
 let extract a secret data len = prf' a secret data len
-
-let kdf     a secret data len = prf' a secret data len
+let kdf a secret data len = prf' a secret data len
